%% LyX 1.6.5 created this file.  For more info, see http://www.lyx.org/.
%% Do not edit unless you really know what you are doing.
\documentclass[english]{article}
\usepackage[T1]{fontenc}
\usepackage[latin9]{inputenc}
\usepackage{esint}
\usepackage{babel}

\begin{document}
\[
\sum_{n=-\infty}^{\infty}f\left(n\right)e^{ikn}=\sum_{m=-\infty}^{\infty}\hat{f}\left(\frac{k}{2\pi}-m\right)\]
Using Dirac delta integral

\[
\sum_{n=-\infty}^{\infty}f\left(n\right)e^{ikn}=\sum_{n=-\infty}^{\infty}\int_{-\infty}^{\infty}\delta\left(x-n\right)f\left(x\right)e^{ikx}dx,\]
which can be reordered to

\[
\sum_{n=-\infty}^{\infty}f\left(n\right)e^{ikn}=\int_{-\infty}^{\infty}f\left(x\right)\sum_{n=-\infty}^{\infty}\delta\left(x-n\right)e^{ikx}dx.\]


Using the relation $\sum_{n=-\infty}^{\infty}\delta\left(x-n\right)=\sum_{m=-\infty}^{\infty}e^{-2\pi mx}$
\[
\sum_{n=-\infty}^{\infty}f\left(n\right)e^{ikn}=\int_{-\infty}^{\infty}f\left(x\right)\sum_{m=-\infty}^{\infty}e^{-2\pi mx}e^{ikx}dx,\]
and reordering the sum\[
\sum_{n=-\infty}^{\infty}f\left(n\right)e^{ikn}=\sum_{m=-\infty}^{\infty}\int_{-\infty}^{\infty}f\left(x\right)e^{i2\pi\left(\frac{k}{2\pi}-m\right)x}dx.\]


Notice that the integral is Fourier transform then we get,\[
\sum_{n=-\infty}^{\infty}f\left(n\right)e^{ikn}=\sum_{m=-\infty}^{\infty}\hat{f}\left(\frac{k}{2\pi}-m\right)\]


Q.E.D.
\end{document}
